{
  "@context": {
    "schema": "http://schema.org/",
    "rdf": "http://www.w3.org/1999/02/22-rdf-syntax-ns#",
    "rdfs": "http://www.w3.org/2000/01/rdf-schema#",
    "bioschemastypesdrafts": "https://discovery.biothings.io/view/bioschemastypesdrafts/"
  },
  "@graph": [
    {
      "@id": "bioschemastypesdrafts:BioSample",
      "@type": "rdfs:Class",
      "rdfs:comment": "A biological material entity that is representative of a whole.\\nComments: Typically samples are intended to be representative of the whole or aspects thereof. Examples of samples include biomedical samples (blood, urine) and plant specimens held at herbaria.\\n\\nVersion: 0.2 \\ncreated by Nick Juty, Sara El-Gebali, Leyla Jael Castro, Helena Schnitzer, Alban Gaignard, Ginger Tsueng, Rita Monteiro and Joana Pauperio. Note, the property `funding` was originally added as `grant`, but was changed to for consistency with schema.org.",
      "rdfs:label": "BioSample",
      "schema:additionalType":"https://bioschemas.org/types#nav-draft",
      "rdfs:subClassOf": {
        "@id": "bioschemastypesdrafts:Sample"
      },
      "schema:schemaVersion": [
        "https://schema.org/docs/releases.html#v23.0"
      ]
    },
    {
      "@id": "bioschemastypesdrafts:dateCollected",
      "@type": "rdf:Property",
      "rdfs:comment": "The date on which the sample was collected.",
      "rdfs:label": "dateCollected",
      "schema:domainIncludes": {"@id": "bioschemastypesdrafts:BioSample"},
      "schema:rangeIncludes": [
        {
          "@id": "schema:Date"
        },
        {
          "@id": "schema:DateTime"
        }
      ]
    },
    {
      "@id": "bioschemastypesdrafts:datePublished",
      "@type": "rdf:Property",
      "rdfs:comment": "The date when the  record of the sample will be made publicly available.",
      "rdfs:label": "datePublished",
      "schema:domainIncludes": {"@id": "bioschemastypesdrafts:BioSample"},
      "schema:rangeIncludes": [
        {
          "@id": "schema:Date"
        },
        {
          "@id": "schema:DateTime"
        }
      ]
    },
    {
      "@id": "bioschemastypesdrafts:submitter",
      "@type": "rdf:Property",
      "rdfs:comment": "The person or organization that registers the sample. ",
      "rdfs:label": "submitter",
      "schema:domainIncludes": {"@id": "bioschemastypesdrafts:BioSample"},
      "schema:rangeIncludes": [
        {
          "@id": "schema:Person"
        },
        {
          "@id": "schema:Organization"
        }
      ]
    },
    {
      "@id": "bioschemastypesdrafts:maintainer",
      "@type": "rdf:Property",
      "rdfs:comment": "The Person or Organization who is responsible for the Sample.",
      "rdfs:label": "maintainer",
      "schema:domainIncludes": {"@id": "bioschemastypesdrafts:BioSample"},
      "schema:rangeIncludes": [
        {
          "@id": "schema:Person"
        },
        {
          "@id": "schema:Organization"
        }
      ]
    },
    {
      "@id": "bioschemastypesdrafts:contributor",
      "@type": "rdf:Property",
      "rdfs:comment": "Person or organization that contributes to the work.",
      "rdfs:label": "contributor",
      "schema:domainIncludes": {"@id": "bioschemastypesdrafts:BioSample"},
      "schema:rangeIncludes": [
        {
          "@id": "schema:Person"
        },
        {
          "@id": "schema:Organization"
        }
      ]
    },
    {
      "@id": "bioschemastypesdrafts:longitude",
      "@type": "rdf:Property",
      "rdfs:comment": "The longitude from which the sample was originally collected. ",
      "rdfs:label": "longitude",
      "schema:domainIncludes": {"@id": "bioschemastypesdrafts:BioSample"},
      "schema:rangeIncludes": [
        {
          "@id": "schema:GeoCoordinates"
        }
      ]
    },
    {
      "@id": "bioschemastypesdrafts:elevation",
      "@type": "rdf:Property",
      "rdfs:comment": "The altitude from which the sample was originally collected. ",
      "rdfs:label": "elevation",
      "schema:domainIncludes": {"@id": "bioschemastypesdrafts:BioSample"},
      "schema:rangeIncludes": [
        {
          "@id": "schema:GeoCoordinates"
        }
      ]
    },
    {
      "@id": "bioschemastypesdrafts:latitude",
      "@type": "rdf:Property",
      "rdfs:comment": "The latitude from which the sample was originally collected. ",
      "rdfs:label": "latitude",
      "schema:domainIncludes": {"@id": "bioschemastypesdrafts:BioSample"},
      "schema:rangeIncludes": [
        {
          "@id": "schema:GeoCoordinates"
        }
      ]
    },
    {
      "@id": "bioschemastypesdrafts:depth",
      "@type": "rdf:Property",
      "rdfs:comment": "The extent downward or inward from the surface from which the sample was originally collected. ",
      "rdfs:label": "depth",
      "schema:domainIncludes": {"@id": "bioschemastypesdrafts:BioSample"},
      "schema:rangeIncludes": [
        {
          "@id": "schema:QuantitativeValue"
        }
      ]
    },
    {
      "@id": "bioschemastypesdrafts:locationOfOrigin",
      "@type": "rdf:Property",
      "rdfs:comment": "The location from which the sample was originally collected.",
      "rdfs:label": "locationOfOrigin",
      "schema:domainIncludes": {"@id": "bioschemastypesdrafts:BioSample"},
      "schema:rangeIncludes": [
        {
          "@id": "schema:GeoCoordinates"
        }
      ]
    },
    {
      "@id": "bioschemastypesdrafts:dateModified",
      "@type": "rdf:Property",
      "rdfs:comment": "Date sample record was last updated.",
      "rdfs:label": "dateModified",
      "schema:domainIncludes": {"@id": "bioschemastypesdrafts:BioSample"},
      "schema:rangeIncludes": [
        {
          "@id": "schema:Date"
        },
        {
          "@id": "schema:DateTime"
        }
      ]
    },
    {
      "@id": "bioschemastypesdrafts:keywords",
      "@type": "rdf:Property",
      "rdfs:comment": "Terms that capture the main subjects e.g. cancer, plant biology.",
      "rdfs:label": "keywords",
      "schema:domainIncludes": {"@id": "bioschemastypesdrafts:BioSample"},
      "schema:rangeIncludes": [
        {
          "@id": "schema:Text"
        }
      ]
    },
    {
      "@id": "bioschemastypesdrafts:alternateIdentifier",
      "@type": "rdf:Property",
      "rdfs:comment": "An additional identifier for the same instance of the resource. ",
      "rdfs:label": "alternateIdentifier",
      "schema:domainIncludes": {"@id": "bioschemastypesdrafts:BioSample"},
      "schema:rangeIncludes": [
        {
          "@id": "schema:Text"
        }
      ]
    },
    {
      "@id": "bioschemastypesdrafts:contactPoint",
      "@type": "rdf:Property",
      "rdfs:comment": "Person or organization that can be contacted for more information or support. ",
      "rdfs:label": "contactPoint",
      "schema:domainIncludes": {"@id": "bioschemastypesdrafts:BioSample"},
      "schema:rangeIncludes": [
        {
          "@id": "schema:Person"
        },
        {
          "@id": "schema:Organization"
        }
      ]
    },
    {
      "@id": "bioschemastypesdrafts:environmentalSystem",
      "@type": "rdf:Property",
      "rdfs:comment": "A category or description of the habitat that describes elements of an ecosystem where the sample was collected.",
      "rdfs:label": "environmentalSystem",
      "schema:domainIncludes": {"@id": "bioschemastypesdrafts:BioSample"},
      "schema:rangeIncludes": [
        {
          "@id": "schema:Text"
        }
      ]
    },
    {
      "@id": "bioschemastypesdrafts:sampleQuantity",
      "@type": "rdf:Property",
      "rdfs:comment": "A numeric value for a measurement of the size  of a sample.",
      "rdfs:label": "sampleQuantity",
      "schema:domainIncludes": {"@id": "bioschemastypesdrafts:BioSample"},
      "schema:rangeIncludes": [
        {
          "@id": "schema:QuantitativeValue"
        }
      ]
    },
    {
      "@id": "bioschemastypesdrafts:processingDate",
      "@type": "rdf:Property",
      "rdfs:comment": "The date the sample was processed or used in a method.",
      "rdfs:label": "processingDate",
      "schema:domainIncludes": {"@id": "bioschemastypesdrafts:BioSample"},
      "schema:rangeIncludes": [
        {
          "@id": "schema:Date"
        },
        {
          "@id": "schema:DateTime"
        }
      ]
    },
    {
      "@id": "bioschemastypesdrafts:sampleState",
      "@type": "rdf:Property",
      "rdfs:comment": "Specify the composition and state of the sample, indicating which form it exisits in, e.g. gas, liquid, solid.",
      "rdfs:label": "sampleState",
      "schema:domainIncludes": {"@id": "bioschemastypesdrafts:BioSample"},
      "schema:rangeIncludes": [
        {
          "@id": "schema:Text"
        }
      ]
    },
    {
      "@id": "bioschemastypesdrafts:sampleType",
      "@type": "rdf:Property",
      "rdfs:comment": "Indicate the type of sample",
      "rdfs:label": "sampleType",
      "schema:domainIncludes": {"@id": "bioschemastypesdrafts:BioSample"},
      "schema:rangeIncludes": [
        {
          "@id": "schema:Text"
        },
        {
          "@id": "schema:URL"
        }
      ]
    },
    {
      "@id": "bioschemastypesdrafts:collectionMethod",
      "@type": "rdf:Property",
      "rdfs:comment": "Provide information about the conditions and methods of acquisition of samples. ",
      "rdfs:label": "collectionMethod",
      "schema:domainIncludes": {"@id": "bioschemastypesdrafts:BioSample"},
      "schema:rangeIncludes": [
        {
          "@id": "schema:Text"
        }
      ]
    },
    {
      "@id": "bioschemastypesdrafts:sampleStorageTemperature",
      "@type": "rdf:Property",
      "rdfs:comment": "Storage condition of the sample.",
      "rdfs:label": "sampleStorageTemperature",
      "schema:domainIncludes": {"@id": "bioschemastypesdrafts:BioSample"},
      "schema:rangeIncludes": [
        {
          "@id": "schema:QualitativeValue"
        }
      ]
    },
    {
      "@id": "bioschemastypesdrafts:sampleProcess",
      "@type": "rdf:Property",
      "rdfs:comment": "The processing technique that was applied to the sample, methods used to prepare the samples.",
      "rdfs:label": "sampleProcess",
      "schema:domainIncludes": {"@id": "bioschemastypesdrafts:BioSample"},
      "schema:rangeIncludes": [
        {
          "@id": "schema:Text"
        }
      ]
    },
    {
      "@id": "bioschemastypesdrafts:experimentalPurpose",
      "@type": "rdf:Property",
      "rdfs:comment": "Describe the planned or executed experimental procedures involving the samples.",
      "rdfs:label": "experimentalPurpose",
      "schema:domainIncludes": {"@id": "bioschemastypesdrafts:BioSample"},
      "schema:rangeIncludes": [
        {
          "@id": "schema:Text"
        }
      ]
    },
    {
      "@id": "bioschemastypesdrafts:instrument",
      "@type": "rdf:Property",
      "rdfs:comment": "Provide description of instruments and devices used.",
      "rdfs:label": "instrument",
      "schema:domainIncludes": {"@id": "bioschemastypesdrafts:BioSample"},
      "schema:rangeIncludes": [
        {
          "@id": "schema:Text"
        },
        {
          "@id": "schema:URL"
        }
      ]
    },
    {
      "@id": "bioschemastypesdrafts:funding",
      "@type": "rdf:Property",
      "rdfs:comment": "Provide funding information.",
      "rdfs:label": "funding",
      "schema:domainIncludes": {"@id": "bioschemastypesdrafts:BioSample"},
      "schema:rangeIncludes": [
        {
          "@id": "schema:Grant"
        }
      ]
    },
    {
      "@id": "bioschemastypesdrafts:project",
      "@type": "rdf:Property",
      "rdfs:comment": "Information on the project.",
      "rdfs:label": "project",
      "schema:domainIncludes": {"@id": "bioschemastypesdrafts:BioSample"},
      "schema:rangeIncludes": [
        {
          "@id": "schema:ResearchProject"
        }
      ]
    },
    {
      "@id": "bioschemastypesdrafts:relatedItem",
      "@type": "rdf:Property",
      "rdfs:comment": "Describe related items including other resources related to the samples.",
      "rdfs:label": "relatedItem",
      "schema:domainIncludes": {"@id": "bioschemastypesdrafts:BioSample"},
      "schema:rangeIncludes": [
        {
          "@id": "schema:Dataset"
        },
        {
          "@id": "schema:ImageObject"
        },
        {
          "@id": "schema:CreativeWork"
        },
        {
          "@id": "schema:Text"
        },
        {
          "@id": "schema:URL"
        }
      ]
    },
    {
      "@id": "bioschemastypesdrafts:isDescribedBy",
      "@type": "rdf:Property",
      "rdfs:comment": "List publications where the sample is mentioned or described.",
      "rdfs:label": "isDescribedBy",
      "schema:domainIncludes": {"@id": "bioschemastypesdrafts:BioSample"},
      "schema:rangeIncludes": [
        {
          "@id": "schema:Article"
        }
      ]
    },
    {
      "@id": "bioschemastypesdrafts:studyTitle",
      "@type": "rdf:Property",
      "rdfs:comment": "Title of the study the samples belong to",
      "rdfs:label": "studyTitle",
      "schema:domainIncludes": {"@id": "bioschemastypesdrafts:BioSample"},
      "schema:rangeIncludes": [
        {
          "@id": "schema:Text"
        }
      ]
    },
    {
      "@id": "bioschemastypesdrafts:studyID",
      "@type": "rdf:Property",
      "rdfs:comment": "Indicate the study ID.",
      "rdfs:label": "studyID",
      "schema:domainIncludes": {"@id": "bioschemastypesdrafts:BioSample"},
      "schema:rangeIncludes": [
        {
          "@id": "schema:Text"
        },
        {
          "@id": "schema:URL"
        }
      ]
    },
    {
      "@id": "bioschemastypesdrafts:sampleAvailability",
      "@type": "rdf:Property",
      "rdfs:comment": "Indicate whether this resource is available for reuse.",
      "rdfs:label": "sampleAvailability",
      "schema:domainIncludes": {"@id": "bioschemastypesdrafts:BioSample"},
      "schema:rangeIncludes": [
        {
          "@id": "schema:Boolean"
        }
      ]
    },
    {
      "@id": "bioschemastypesdrafts:accessConditions",
      "@type": "rdf:Property",
      "rdfs:comment": "Sample access statement outlining conditions/requirements need to be fulfilled before access to the sample is granted.",
      "rdfs:label": "accessConditions",
      "schema:domainIncludes": {"@id": "bioschemastypesdrafts:BioSample"},
      "schema:rangeIncludes": [
        {
          "@id": "schema:Text"
        }
      ]
    },
    {
      "@id": "bioschemastypesdrafts:ethics",
      "@type": "rdf:Property",
      "rdfs:comment": "Indicate which ethics policies are associated with the sample.",
      "rdfs:label": "ethics",
      "schema:domainIncludes": {"@id": "bioschemastypesdrafts:BioSample"},
      "schema:rangeIncludes": [
        {
          "@id": "schema:Text"
        }
      ]
    },
    {
      "@id": "bioschemastypesdrafts:scientificName",
      "@type": "rdf:Property",
      "rdfs:comment": "The full scientific name (order, family, subfamily,  genus,specificEpithet).",
      "rdfs:label": "scientificName",
      "schema:domainIncludes": {"@id": "bioschemastypesdrafts:BioSample"},
      "schema:rangeIncludes": [
        {
          "@id": "schema:Text"
        }
      ]
    },
    {
      "@id": "bioschemastypesdrafts:anatomicalSystem",
      "@type": "rdf:Property",
      "rdfs:comment": "An anatomical system is a group of anatomical structures that work together to perform a certain task. Can include circulatory, digestive, endocrine, immune and other systems",
      "rdfs:label": "anatomicalSystem",
      "schema:domainIncludes": {"@id": "bioschemastypesdrafts:BioSample"},
      "schema:rangeIncludes": [
        {
          "@id": "schema:AnatomicalSystem"
        }
      ]
    },
    {
      "@id": "bioschemastypesdrafts:organ",
      "@type": "rdf:Property",
      "rdfs:comment": "Anatomical structure that performs a specific function or group of function.",
      "rdfs:label": "organ",
      "schema:domainIncludes": {"@id": "bioschemastypesdrafts:BioSample"},
      "schema:rangeIncludes": [
        {
          "@id": "schema:AnatomicalStructure"
        }
      ]
    },
    {
      "@id": "bioschemastypesdrafts:tissue",
      "@type": "rdf:Property",
      "rdfs:comment": "Indicate the tissue from which the sample was collected.",
      "rdfs:label": "tissue",
      "schema:domainIncludes": {"@id": "bioschemastypesdrafts:BioSample"},
      "schema:rangeIncludes": [
        {
          "@id": "schema:AnatomicalStructure"
        }
      ]
    },
    {
      "@id": "bioschemastypesdrafts:sex",
      "@type": "rdf:Property",
      "rdfs:comment": "The biological sex of the individual from which the sample was obtained.",
      "rdfs:label": "sex",
      "schema:domainIncludes": {"@id": "bioschemastypesdrafts:BioSample"},
      "schema:rangeIncludes": [
        {
          "@id": "schema:Text"
        }
      ]
    },
    {
      "@id": "bioschemastypesdrafts:developmentalStage",
      "@type": "rdf:Property",
      "rdfs:comment": "A temporal subdivision of a developmental process, indicating the age or stage of the object when the sample was created.",
      "rdfs:label": "developmentalStage",
      "schema:domainIncludes": {"@id": "bioschemastypesdrafts:BioSample"},
      "schema:rangeIncludes": [
        {
          "@id": "schema:Text"
        }
      ]
    },
    {
      "@id": "bioschemastypesdrafts:relationshipType",
      "@type": "rdf:Property",
      "rdfs:comment": "Describe the relationship to other entities or organisms e.g. parent, sibling, symbiont.",
      "rdfs:label": "relationshipType",
      "schema:domainIncludes": {"@id": "bioschemastypesdrafts:BioSample"},
      "schema:rangeIncludes": [
        {
          "@id": "schema:Text"
        }
      ]
    }
  ]
}
